haskell ffi stubs for use in raaz for all primitives.

src/Verse/CryptoLib/blake2b/c/portable.v
@@ -111,6 +111,17 @@ Definition iterator   : Compile.programLine := recover (blake2bIter).
 Definition lastchunk  : Compile.programLine := recover (blake2bLast).
 Definition program := verseC [iterator; lastchunk].
 
+Require Import Verse.FFI.Raaz.
+Require Import Verse.FFI.Raaz.Target.C.
+
+Definition raazFFI
+  := ffi [ iterator verse_blake2b_c_portable_iter
+                    Blake2b.Block
+                    Blake2b.paramIterator;
+           function verse_blake2b_c_portable_last
+                    Blake2b.paramLastBlock
+         ].
+
 (*
 
 Require Import Verse.Print.
