src/Verse/CryptoLib/blake2s/c/portable.v
@@ -113,6 +113,17 @@ Definition iterator   : Compile.programLine := recover (blake2sIter).
 Definition lastchunk  : Compile.programLine := recover (blake2sLast).
 Definition program := verseC [iterator; lastchunk].
 
+Require Import Verse.FFI.Raaz.
+Require Import Verse.FFI.Raaz.Target.C.
+
+Definition raazFFI
+  := ffi [ iterator verse_blake2s_c_portable_iter
+                    Blake2s.Block
+                    Blake2s.paramIterator;
+           function verse_blake2s_c_portable_last
+                    Blake2s.paramLastBlock
+         ].
+
 (*
 
 Require Import Verse.Print.
