src/Verse/CryptoLib/poly1305/c/portable.v
@@ -858,6 +858,23 @@ Definition program := verseC [ incrementalI;
                              ].
 
 
+Require Import Verse.FFI.Raaz.
+Require Import Verse.FFI.Raaz.Target.C.
+
+Definition raazFFI
+  := ffi [ iterator verse_poly1305_c_portable_incremental
+                    Block
+                    Internal.paramsIncremental;
+           iterator verse_poly1305_c_portable_blockmac
+                    Block
+                    Internal.paramsBlockMac;
+           iterator verse_poly1305_c_portable_clamp
+                    Internal.Array128
+                    [];
+           function verse_poly1305_c_portable_partialmac
+                    Internal.paramsPartialMac
+         ].
+
 
 (*
 
