src/Verse/CryptoLib/sha256/c/portable.v
@@ -133,6 +133,16 @@ Require Import Verse.Error.
 Definition iterator : Compile.programLine := recover sha256iter.
 Definition program := verseC [iterator].
 
+Require Import Verse.FFI.Raaz.
+Require Import Verse.FFI.Raaz.Target.C.
+
+Definition raazFFI
+  := ffi [ iterator verse_sha256_c_portable
+                    SHA256.Block
+                    SHA256.parameters
+         ].
+
+
 (*
 
 Require Import Verse.Print.
